README.md
@@ -1,7 +1,7 @@
 [![Build Status](https://travis-ci.org/SEL4PROJ/jormungand.svg?branch=master)](https://travis-ci.org/SEL4PROJ/jormungand)
 
 This repository contains the supporting Isabelle/HOL theories
-for the paper "Walking Backwards and Forwards with Separation Logic".
+for the paper "Backwards and Forwards with Separation Logic".
 
 Hoare_Sep_Tactics/ contains the main relevant theory files, they are
 
